generic/Zeta.TimeKey.fsti
@@ -1,0 +1,29 @@
+module Zeta.TimeKey
+
+open Zeta.Time
+open Zeta.Key
+
+let timestamp_key = timestamp & base_key
+
+(* < *)
+let lt (tk1 tk2: timestamp_key)
+  = let t1,k1 = tk1 in
+    let t2,k2 = tk2 in
+    t1 `ts_lt` t2 || t1 = t2 && k1 `Zeta.BinTree.lt` k2
+
+(* <= *)
+let lte tk1 tk2 = tk1 = tk2 || tk1 `lt` tk2
+
+(* > *)
+let gt tk1 tk2 = tk2 `lt` tk1
+
+(* >= *)
+let gte tk1 tk2 = not (tk1 `lt` tk2)
+
+val lt_is_total (tk1 tk2: timestamp_key)
+  : Lemma (ensures (tk1 = tk2 /\ ~ (tk1 `lt` tk2) /\ ~ (tk2 `lt` tk1) \/
+                    tk1 <> tk2 /\ (tk1 `lt` tk2 \/ tk2 `lt` tk1)))
+          [SMTPat (tk1 `lt` tk2)]
+
+val lt_is_transitive (tk1 tk2 tk3: _)
+  : Lemma (ensures (tk1 `lt` tk2 ==> tk2 `lt` tk3 ==> tk1 `lt` tk3))
